restructuring

FxyLang/Reasoning/Progression.lean
@@ -4,47 +4,11 @@
   Authors: Arthur Paulino
 -/
 
-import FxyLang.Implementation.Execution
-import Lean
-
-def State.isProg : State → Bool
-  | prog .. => true
-  | _       => false
-
-def State.isEnd : State → Bool
-  | done  .. => true
-  | error .. => true
-  | _        => false
-
-def State.stepN : State → Nat → State
-  | s, 0     => s
-  | s, n + 1 => s.step.stepN n
-
-notation s "^" "[" n "]" => State.stepN s n
-
-theorem State.stepNComp : (s^[n₁])^[n₂] = s^[n₁ + n₂] := by
-  induction n₁ generalizing s with
-  | zero => simp [stepN]
-  | succ n hi =>
-    have := @hi (s^[1])
-    simp only [stepN] at this
-    rw [stepN, this]
-    have : n.succ + n₂ = (n + n₂).succ := by
-      simp only [Nat.add_comm, Nat.add_assoc, Nat.add_left_comm]; rfl
-    rw [this, stepN]
-
-theorem State.doneLoop : done v c^[n] = done v c := by
-  induction n with
-  | zero      => rw [stepN]
-  | succ _ hi => rw [stepN, step]; exact hi
-
-theorem State.errorLoop : error t v c^[n] = error t v c := by
-  induction n with
-  | zero      => rw [stepN]
-  | succ _ hi => rw [stepN, step]; exact hi
+import FxyLang.Reasoning.Defs
 
 open Lean.Parser.Tactic in
-syntax "step_induction " ident (" using " term,+)? (" with " simpLemma)? :tactic
+syntax "step_induction " ident (" using " term,+)?
+  (" with " simpLemma)? : tactic
 
 open Lean.Elab.Tactic in
 set_option hygiene false in
@@ -93,7 +57,10 @@ theorem State.retProgression :
     cases h : v₂.binOp v o with
     | error => exact ⟨1, by simp [stepN, step, h, isEnd]⟩
     | ok v' => step_induction hi using v', c with h
-  | binOp₁ o e k hi => sorry
+  | binOp₁ o e k hi =>
+    sorry
+    -- cases @exprProgression e c (Continuation.binOp₂ o v k) with | intro n h =>
+    -- exact ⟨n + 1, by simp only [stepN, step]; exact h⟩
   | app e es k hi =>
     cases v with
     | lam lm =>
@@ -107,8 +74,8 @@ theorem State.retProgression :
     | _ => exact ⟨1, by simp [stepN, step, isEnd]⟩
 
 open Lean.Parser.Tactic in
-syntax "step_ret " num " using " term ", " term ", "
-  term (" with " simpLemma)? : tactic
+syntax "step_ret " num " using " term ", " term ", " term
+  (" with " simpLemma)? : tactic
 
 open Lean.Elab.Tactic in
 set_option hygiene false in
@@ -181,129 +148,22 @@ theorem State.exprProgression :
     | app e es k => step_ret 1 using .lam l, c, .app e es k
     | block c' k => step_ret 1 using .lam l, c, .block c' k
   | app e es =>
-    have := @exprProgression e c (.app e es k)
-    cases this with | intro n h =>
-    exact ⟨n + 1, by simp [stepN, step]; exact h⟩
+    sorry
+    -- cases @exprProgression e c (.app e es k) with | intro n h =>
+    -- exact ⟨n + 1, by rw [stepN, step]; exact h⟩
   | unOp o e =>
-    have := @exprProgression e c (.unOp o e k)
-    cases this with | intro n h =>
-    exact ⟨n + 1, by simp [stepN, step]; exact h⟩
+    sorry
+    -- cases @exprProgression e c (.unOp o e k) with | intro n h =>
+    -- exact ⟨n + 1, by rw [stepN, step]; exact h⟩
   | binOp o e₁ e₂ =>
-    have := @exprProgression e₁ c (.binOp₁ o e₂ k)
-    cases this with | intro n h =>
-    exact ⟨n + 1, by simp [stepN, step]; exact h⟩
-decreasing_by sorry
+    sorry
+    -- cases @exprProgression e₁ c (.binOp₁ o e₂ k) with | intro n h =>
+    -- exact ⟨n + 1, by rw [stepN, step]; exact h⟩
 
-open State in
-theorem Progression : ∃ n, (s^[n]).isEnd ∨ (s^[n]).isProg := by
+theorem State.Progression : ∃ n, (s^[n]).isEnd ∨ (s^[n]).isProg := by
   cases s with
   | prog  => exact ⟨0, by simp [stepN, isProg]⟩
   | done  => exact ⟨0, by simp [stepN,  isEnd]⟩
   | error => exact ⟨0, by simp [stepN,  isEnd]⟩
   | ret  v c k => exact retProgression
   | expr e c k => exact exprProgression
-
-def State.reachesWith (s₁ s₂ : State) (f : State → Prop) : Prop :=
-  ∃ n, s₁^[n] = s₂ ∧ ∀ i, i ≤ n → f (s₁^[i])
-
-inductive Continuation.derives (k₀ : Continuation) : Continuation → Prop
-  | byId     : derives k₀ k₀
-  | bySeq    : derives k₀ k → derives k₀ (.seq      _ k)
-  | byDecl   : derives k₀ k → derives k₀ (.decl     _ k)
-  | byFork   : derives k₀ k → derives k₀ (.fork _ _ _ k)
-  | byLoop   : derives k₀ k → derives k₀ (.loop   _ _ k)
-  | byUnOp   : derives k₀ k → derives k₀ (.unOp   _ _ k)
-  | byBinOp₁ : derives k₀ k → derives k₀ (.binOp₁ _ _ k)
-  | byBinOp₂ : derives k₀ k → derives k₀ (.binOp₂ _ _ k)
-  | byApp    : derives k₀ k → derives k₀ (.app    _ _ k)
-  | byBlock  : derives k₀ k → derives k₀ (.block    _ k)
-  | byPrint  : derives k₀ k → derives k₀ (.print      k)
-
-open Continuation.derives
-
-def State.derivesFrom (k₀ : Continuation) : State → Prop
-| ret  _ _ k => k₀.derives k
-| prog _ _ k => k₀.derives k
-| expr _ _ k => k₀.derives k
-| error ..   => False
-| done  ..   => False
-
-def bigStep (c : Context) (p : Program) (c' : Context) (v : Value) : Prop :=
-  ∀ k, (State.prog p c k).reachesWith (.ret v c' k) (·.derivesFrom k)
-
-notation "⟦" c ", " p "⟧" " » " "⟦" c' ", " v "⟧" => bigStep c p c' v
-
-theorem State.skip : ⟦c, .skip⟧ » ⟦c, .nil⟧ := by
-  intro k
-  refine ⟨1, ?_⟩
-  simp [stepN, step]
-  intro i hᵢ
-  cases i with
-  | zero => rw [stepN]; exact byId
-  | succ i =>
-    cases i with
-    | zero => rw [stepN]; exact byId
-    | succ i =>
-    have : i.succ.succ > 1 := by
-      by_cases h : i.succ.succ ≤ 1
-      · by_cases h' : i.succ.succ > 1
-        · exact h'
-        · contradiction
-      · exact Nat.gt_of_not_le h  
-    contradiction
-
--- set_option hygiene false in
-macro "big_step " h:ident " with "
-    k:ident n:ident h₁:ident h₂:ident : tactic => do
-  `(tactic| have $k:ident : Continuation := default;
-            have $h₁:ident := $h:ident $k:ident;
-            cases $h₁:ident with | intro $n:ident FOO__ => ?_;
-            have $h₁:ident := FOO__.1;
-            have $h₂:ident := FOO__.2;
-            clear FOO__)
-
-open Lean.Elab.Tactic in
-set_option hygiene false in
-elab "small_step " n:ident " at " h:ident : tactic => do
-  evalTactic $ ←`(tactic| cases $n:ident with
-                          | zero => simp [step, stepN] at $h:ident
-                          | succ $n:ident => ?_)
-  evalTactic $ ←`(tactic| simp [step, stepN] at $h:ident)
-
-theorem State.eval (h : ⟦c, .eval e⟧ » ⟦c', v⟧) : c = c' := by
-  big_step h with k n h₁ h₂
-  cases e with
-  | lit l =>
-    small_step n at h₁
-    small_step n at h₁
-    sorry
-  | _ => sorry
-
-theorem State.decl (h : ⟦c, .decl nm p⟧ » ⟦c', v⟧) : c' = c.insert nm v := by
-  big_step h with k n h₁ h₂
-  sorry
-
-def State.canContinue : State → Bool
-  | ret  .. => true
-  | expr .. => true
-  | prog .. => true
-  | _       => false
-
-theorem State.derivesForward {s : State}
-  (hs : s.derivesFrom k) (hc : s.canContinue) :
-    s.step.derivesFrom k := by
-  sorry
-
-theorem State.reachDeterministic'
-  (h : (ret v₁ c₁ k).reachesWith (ret v₂ c₂ k) (·.derivesFrom k)) :
-    v₁ = v₂ ∧ c₁ = c₂ := by
-  sorry
-
-theorem reachDeterministic {s: State} 
-  (h₁ : s.reachesWith (.ret v₁ c₁ k) (·.derivesFrom k))
-  (h₂ : s.reachesWith (.ret v₂ c₂ k) (·.derivesFrom k)) :
-    v₁ = v₂ ∧ c₁ = c₂ := by
-  sorry
-
-theorem Determinism (h₁ : ⟦c, p⟧ » ⟦c₁, v₁⟧) (h₂ : ⟦c, p⟧ » ⟦c₂, v₂⟧) :
-  v₁ = v₂ ∧ c₁ = c₂ := reachDeterministic (h₁ default) (h₂ default)
