FxyLang/Reasoning/BigStep.lean
@@ -1,0 +1,59 @@
+/-
+  Copyright (c) 2022 Arthur Paulino. All rights reserved.
+  Released under Apache 2.0 license as described in the file LICENSE.
+  Authors: Arthur Paulino
+-/
+
+import FxyLang.Reasoning.Defs
+
+open Continuation.extends
+
+theorem State.skip : ⟦c, .skip⟧ » ⟦c, .nil⟧ := by
+  intro k
+  refine ⟨1, ?_⟩
+  simp [stepN, step]
+  intro i hᵢ
+  cases i with
+  | zero => rw [stepN]; exact byId
+  | succ i =>
+    cases i with
+    | zero => rw [stepN]; exact byId
+    | succ i =>
+    have : i.succ.succ > 1 := by
+      by_cases h : i.succ.succ ≤ 1
+      · by_cases h' : i.succ.succ > 1
+        · exact h'
+        · contradiction
+      · exact Nat.gt_of_not_le h  
+    contradiction
+
+-- set_option hygiene false in
+macro "big_step " h:ident " with "
+    k:ident n:ident h₁:ident h₂:ident : tactic => do
+  `(tactic| have $k:ident : Continuation := default;
+            have $h₁:ident := $h:ident $k:ident;
+            cases $h₁:ident with | intro $n:ident FOO__ => ?_;
+            have $h₁:ident := FOO__.1;
+            have $h₂:ident := FOO__.2;
+            clear FOO__)
+
+open Lean.Elab.Tactic in
+set_option hygiene false in
+elab "small_step " n:ident " at " h:ident : tactic => do
+  evalTactic $ ←`(tactic| cases $n:ident with
+                          | zero => simp [step, stepN] at $h:ident
+                          | succ $n:ident => ?_)
+  evalTactic $ ←`(tactic| simp [step, stepN] at $h:ident)
+
+theorem State.eval (h : ⟦c, .eval e⟧ » ⟦c', v⟧) : c = c' := by
+  big_step h with k n h₁ h₂
+  cases e with
+  | lit l =>
+    small_step n at h₁
+    small_step n at h₁
+    sorry
+  | _ => sorry
+
+theorem State.decl (h : ⟦c, .decl nm p⟧ » ⟦c', v⟧) : c' = c.insert nm v := by
+  big_step h with k n h₁ h₂
+  sorry
