FxyLang/Reasoning/Defs.lean
@@ -1,0 +1,70 @@
+/-
+  Copyright (c) 2022 Arthur Paulino. All rights reserved.
+  Released under Apache 2.0 license as described in the file LICENSE.
+  Authors: Arthur Paulino
+-/
+
+import FxyLang.Implementation.Execution
+import Lean
+
+def State.isProg : State → Bool
+  | prog .. => true
+  | _       => false
+
+def State.isEnd : State → Bool
+  | done  .. => true
+  | error .. => true
+  | _        => false
+
+def State.stepN : State → Nat → State
+  | s, 0     => s
+  | s, n + 1 => s.step.stepN n
+
+notation s "^" "[" n "]" => State.stepN s n
+
+def State.reachesWith (s₁ s₂ : State) (f : State → Prop) : Prop :=
+  ∃ n, s₁^[n] = s₂ ∧ ∀ i, i ≤ n → f (s₁^[i])
+
+inductive Continuation.extends (k : Continuation) : Continuation → Prop
+  | byId     : «extends» k k
+  | bySeq    : «extends» k k' → «extends» k (.seq      _ k')
+  | byDecl   : «extends» k k' → «extends» k (.decl     _ k')
+  | byFork   : «extends» k k' → «extends» k (.fork _ _ _ k')
+  | byLoop   : «extends» k k' → «extends» k (.loop   _ _ k')
+  | byUnOp   : «extends» k k' → «extends» k (.unOp   _ _ k')
+  | byBinOp₁ : «extends» k k' → «extends» k (.binOp₁ _ _ k')
+  | byBinOp₂ : «extends» k k' → «extends» k (.binOp₂ _ _ k')
+  | byApp    : «extends» k k' → «extends» k (.app    _ _ k')
+  | byBlock  : «extends» k k' → «extends» k (.block    _ k')
+  | byPrint  : «extends» k k' → «extends» k (.print      k')
+
+def Continuation.height : Continuation → Nat
+  | exit         => 1
+  | seq      _ k => k.height + 1
+  | decl     _ k => k.height + 1
+  | fork _ _ _ k => k.height + 1
+  | loop   _ _ k => k.height + 1
+  | unOp   _ _ k => k.height + 1
+  | binOp₁ _ _ k => k.height + 1
+  | binOp₂ _ _ k => k.height + 1
+  | app    _ _ k => k.height + 1
+  | block    _ k => k.height + 1
+  | print      k => k.height + 1
+
+def State.extends (k₀ : Continuation) : State → Prop
+| ret  _ _ k => k₀.extends k
+| prog _ _ k => k₀.extends k
+| expr _ _ k => k₀.extends k
+| error ..   => True
+| done  ..   => False
+
+def State.canContinue : State → Bool
+  | ret  .. => true
+  | expr .. => true
+  | prog .. => true
+  | _       => false
+
+def bigStep (c : Context) (p : Program) (c' : Context) (v : Value) : Prop :=
+  ∀ k, (State.prog p c k).reachesWith (.ret v c' k) (·.«extends» k)
+
+notation "⟦" c ", " p "⟧" " » " "⟦" c' ", " v "⟧" => bigStep c p c' v
