FxyLang/Reasoning/Determinism.lean
@@ -1,0 +1,26 @@
+/-
+  Copyright (c) 2022 Arthur Paulino. All rights reserved.
+  Released under Apache 2.0 license as described in the file LICENSE.
+  Authors: Arthur Paulino
+-/
+
+import FxyLang.Reasoning.Defs
+
+theorem State.extendsForward {s : State}
+  (hs : s.extends k) (hc : s.canContinue) :
+    s.step.extends k := by
+  sorry
+
+theorem State.reachDeterministic'
+  (h : (ret v₁ c₁ k).reachesWith (ret v₂ c₂ k) (·.«extends» k)) :
+    v₁ = v₂ ∧ c₁ = c₂ := by
+  sorry
+
+theorem reachDeterministic {s: State} 
+  (h₁ : s.reachesWith (.ret v₁ c₁ k) (·.«extends» k))
+  (h₂ : s.reachesWith (.ret v₂ c₂ k) (·.«extends» k)) :
+    v₁ = v₂ ∧ c₁ = c₂ := by
+  sorry
+
+theorem Determinism (h₁ : ⟦c, p⟧ » ⟦c₁, v₁⟧) (h₂ : ⟦c, p⟧ » ⟦c₂, v₂⟧) :
+  v₁ = v₂ ∧ c₁ = c₂ := reachDeterministic (h₁ default) (h₂ default)
